ironfleet/src/Dafny/Distributed/Protocol/RSL/FailureProof/Common/definitions.i.dfy
@@ -1,0 +1,70 @@
+include "../TimestampedRslSystem.i.dfy"
+include "../../CommonProof/Constants.i.dfy"
+
+module Common_Definitions {
+import opened TimestampedRslSystem_i
+import opened CommonProof__Constants_i
+
+
+
+/*****************************************************************************************
+*                                     Definitions                                        *
+*****************************************************************************************/
+
+
+predicate RslConsistency(ts:TimestampedRslState)
+{
+    ConstantsAllConsistentInv(UntimestampRslState(ts))
+        && WellFormedLConfiguration(ts.constants.config)
+}
+
+
+predicate ServersAreNotClients(ts:TimestampedRslState)
+{
+  forall id :: id in ts.constants.config.clientIds && id in ts.constants.config.replica_ids
+    ==> false
+}
+
+predicate RequestBatchSrcInClientIds(ts:TimestampedRslState, v:RequestBatch)
+{
+  forall r :: r in v ==> r.client in ts.constants.config.clientIds
+}
+
+predicate LeaderSet1bContainsRequest(ts:TimestampedRslState) 
+    requires |ts.t_replicas| > 2
+{
+    var r := ts.t_replicas[1].v.replica;
+    && LProposerCanNominateUsingOperationNumber(r.proposer, r.acceptor.log_truncation_point, r.proposer.next_operation_number_to_propose)
+    && !LAllAcceptorsHadNoProposal(r.proposer.received_1b_packets, r.proposer.next_operation_number_to_propose)
+}
+
+predicate IsNew2aPacket(pkt:TimestampedRslPacket, opn:OperationNumber) {
+    && pkt.msg.v.RslMessage_2a?
+    && pkt.msg.v.bal_2a == Ballot(1, 1)
+    && pkt.msg.v.opn_2a == opn
+}
+
+predicate IsNew2bPacket(pkt:TimestampedRslPacket, opn:OperationNumber) {
+    && pkt.msg.v.RslMessage_2b?
+    && pkt.msg.v.bal_2b == Ballot(1, 1)
+    && pkt.msg.v.opn_2b == opn
+}
+
+predicate IsNewReplyPacket(ts:TimestampedRslState, pkt:TimestampedRslPacket) 
+    requires |ts.t_replicas| > 2
+    requires RslConsistency(ts)
+{
+    && pkt.msg.v.RslMessage_Reply?
+    && pkt.src == ts.constants.config.replica_ids[1]
+}
+
+function Get2bCount(s:LReplica, opn:OperationNumber, ballot:Ballot) : int
+{
+  if opn !in s.learner.unexecuted_learner_state then
+    0
+  else
+    |s.learner.unexecuted_learner_state[opn].received_2b_message_senders|
+}
+
+
+}
